NAND_Hoare.thy
@@ -14,16 +14,79 @@ begin
 
 subsection \<open>Proving @{term "nand3"}: NAND with transport delay \<close>
 
-text \<open>type for the signals\<close>
+lemma beval_world_raw2_type:
+  assumes "wityping \<Gamma>' (snd tw)"
+  assumes "beval_world_raw2 tw (Bnand (Bsig A) (Bsig B)) v"
+  shows   "type_of v = \<Gamma>' A"
+proof -
+  have "beval_world_raw (snd tw) (fst tw) (Bnand (Bsig A) (Bsig B)) v"
+    using assms(2) unfolding beval_world_raw2_def by auto
+  then obtain \<sigma> \<gamma> \<theta> where "\<sigma> = state_of_world (snd tw) (fst tw)" and
+                          "\<gamma> = event_of_world (snd tw) (fst tw)" and
+                          "\<theta> = derivative_hist_raw (snd tw) (fst tw)" and
+                          "fst tw, \<sigma>, \<gamma>, \<theta>, (fst (snd tw)) \<turnstile> (Bnand (Bsig A) (Bsig B)) \<longrightarrow>\<^sub>b v"
+    using beval_world_raw_cases by force
+  have "styping \<Gamma>' \<sigma>"
+    using wityping_ensure_styping
+    by (simp add: wityping_ensure_styping \<open>\<sigma> = state_of_world (snd tw) (get_time tw)\<close> assms(1))
+  moreover have "ttyping \<Gamma>' \<theta>"
+    using wityping_ensure_ttyping
+    by (simp add: wityping_ensure_ttyping \<open>\<theta> = derivative_hist_raw (snd tw) (get_time tw)\<close> assms(1))
+  moreover have "styping \<Gamma>' (fst (snd tw))"
+    using assms(1) unfolding wityping_def by blast
+  moreover have "\<Gamma>' A = \<Gamma>' B"
+    apply(rule beval_cases(9)[OF `fst tw, \<sigma>, \<gamma>, \<theta>, (fst (snd tw)) \<turnstile> (Bnand (Bsig A) (Bsig B)) \<longrightarrow>\<^sub>b v`])
+    apply (metis beval_raw_preserve_well_typedness bexp_wt.intros(3) calculation(1) calculation(2) calculation(3) type_of.simps(1))
+    by (metis (full_types) beval_cases(1) calculation(1) styping_def type_of.simps(2))
+  moreover have "bexp_wt \<Gamma>' (Bnand (Bsig A) (Bsig B)) (\<Gamma>' A)"
+    by (metis bexp_wt.intros(3) bexp_wt.intros(9) calculation(4))
+  ultimately show ?thesis
+    using beval_raw_preserve_well_typedness
+    by (metis \<open>get_time tw , \<sigma> , \<gamma> , \<theta>, get_time (snd tw) \<turnstile> Bnand (Bsig A) (Bsig B) \<longrightarrow>\<^sub>b v\<close>)
+qed
 
-fun \<Gamma> :: "sig tyenv" where
-  "\<Gamma> A = Bty" | "\<Gamma> B = Bty" | "\<Gamma> C = Bty"
+lemma beval_world_raw2_typeB:
+  assumes "wityping \<Gamma>' (snd tw)"
+  assumes "beval_world_raw2 tw (Bnand (Bsig A) (Bsig B)) v"
+  shows   "type_of v = \<Gamma>' B"
+proof -
+  have "beval_world_raw (snd tw) (fst tw) (Bnand (Bsig A) (Bsig B)) v"
+    using assms(2) unfolding beval_world_raw2_def by auto
+  then obtain \<sigma> \<gamma> \<theta> where "\<sigma> = state_of_world (snd tw) (fst tw)" and
+                          "\<gamma> = event_of_world (snd tw) (fst tw)" and
+                          "\<theta> = derivative_hist_raw (snd tw) (fst tw)" and
+                          "fst tw, \<sigma>, \<gamma>, \<theta>, (fst (snd tw)) \<turnstile> (Bnand (Bsig A) (Bsig B)) \<longrightarrow>\<^sub>b v"
+    using beval_world_raw_cases by force
+  have "styping \<Gamma>' \<sigma>"
+    using wityping_ensure_styping
+    by (simp add: wityping_ensure_styping \<open>\<sigma> = state_of_world (snd tw) (get_time tw)\<close> assms(1))
+  moreover have "ttyping \<Gamma>' \<theta>"
+    using wityping_ensure_ttyping
+    by (simp add: wityping_ensure_ttyping \<open>\<theta> = derivative_hist_raw (snd tw) (get_time tw)\<close> assms(1))
+  moreover have "styping \<Gamma>' (fst (snd tw))"
+    using assms(1) unfolding wityping_def by blast
+  moreover have "\<Gamma>' A = \<Gamma>' B"
+    apply(rule beval_cases(9)[OF `fst tw, \<sigma>, \<gamma>, \<theta>, (fst (snd tw)) \<turnstile> (Bnand (Bsig A) (Bsig B)) \<longrightarrow>\<^sub>b v`])
+    apply (metis beval_raw_preserve_well_typedness bexp_wt.intros(3) calculation(1) calculation(2) calculation(3) type_of.simps(1))
+    by (metis (full_types) beval_cases(1) calculation(1) styping_def type_of.simps(2))
+  moreover have "bexp_wt \<Gamma>' (Bnand (Bsig A) (Bsig B)) (\<Gamma>' B)"
+    by (metis bexp_wt.intros(3) bexp_wt.intros(9) calculation(4))
+  ultimately show ?thesis
+    using beval_raw_preserve_well_typedness
+    by (metis \<open>get_time tw , \<sigma> , \<gamma> , \<theta>, get_time (snd tw) \<turnstile> Bnand (Bsig A) (Bsig B) \<longrightarrow>\<^sub>b v\<close>)
+qed
+
+abbreviation "bval_of_wline tw sig n \<equiv> bval_of (wline_of tw sig n)"
+abbreviation "lof_wline tw sig n \<equiv> lval_of (wline_of tw sig n)"
+
+locale scalar_type_nand3 =
+  fixes \<Gamma> :: "sig tyenv"
+  assumes "\<Gamma> A = Bty" and "\<Gamma> B = Bty" and "\<Gamma> C = Bty"
+begin
 
 text \<open>Invariant for NAND: at all times @{term "i"} less than @{term "fst tw :: nat"}, the signal
 @{term "C :: sig"} at @{term "i + 1"} should be the NAND value of @{term "A :: sig"} and
 @{term "B :: sig"} at time @{term "i"}.\<close>
-
-abbreviation "bval_of_wline tw sig n \<equiv> bval_of (wline_of tw sig n)"
 
 definition nand_inv :: "sig assn2" where
   "nand_inv \<equiv> (\<lambda>tw. \<forall>i < fst tw. bval_of_wline tw C (i + 1) \<longleftrightarrow> \<not> (bval_of_wline tw A i \<and> bval_of_wline tw B i))"
@@ -118,38 +181,11 @@ proof -
     unfolding nand_inv_def by auto
 qed
 
-lemma beval_world_raw2_type:
-  assumes "wityping \<Gamma> (snd tw)"
-  assumes "beval_world_raw2 tw (Bnand (Bsig A) (Bsig B)) v"
-  shows   "type_of v = Bty"
-proof -
-  have "beval_world_raw (snd tw) (fst tw) (Bnand (Bsig A) (Bsig B)) v"
-    using assms(2) unfolding beval_world_raw2_def by auto
-  then obtain \<sigma> \<gamma> \<theta> where "\<sigma> = state_of_world (snd tw) (fst tw)" and
-                          "\<gamma> = event_of_world (snd tw) (fst tw)" and
-                          "\<theta> = derivative_hist_raw (snd tw) (fst tw)" and
-                          "fst tw, \<sigma>, \<gamma>, \<theta>, (fst (snd tw)) \<turnstile> (Bnand (Bsig A) (Bsig B)) \<longrightarrow>\<^sub>b v"
-    using beval_world_raw_cases by force
-  have "styping \<Gamma> \<sigma>"
-    using wityping_ensure_styping
-    by (simp add: wityping_ensure_styping \<open>\<sigma> = state_of_world (snd tw) (get_time tw)\<close> assms(1))
-  moreover have "ttyping \<Gamma> \<theta>"
-    using wityping_ensure_ttyping
-    by (simp add: wityping_ensure_ttyping \<open>\<theta> = derivative_hist_raw (snd tw) (get_time tw)\<close> assms(1))
-  moreover have "styping \<Gamma> (fst (snd tw))"
-    using assms(1) unfolding wityping_def by blast
-  moreover have "bexp_wt \<Gamma> (Bnand (Bsig A) (Bsig B)) Bty"
-    by (metis \<Gamma>.elims bexp_wt.intros(3) bexp_wt.intros(9))
-  ultimately show ?thesis
-    using beval_raw_preserve_well_typedness
-    by (metis \<open>get_time tw , \<sigma> , \<gamma> , \<theta>, get_time (snd tw) \<turnstile> Bnand (Bsig A) (Bsig B) \<longrightarrow>\<^sub>b v\<close>)
-qed
-
 lemma nand_seq_hoare_next_time:
   "\<turnstile> [\<lambda>tw. nand_inv tw \<and> wityping \<Gamma> (snd tw)] (Bassign_trans C (Bnand (Bsig A) (Bsig B)) 1) [\<lambda>tw. nand_inv (next_time_world tw, snd tw) \<and> wityping \<Gamma> (snd tw)]"
   apply (rule Conseq2[where Q="\<lambda>tw. nand_inv (next_time_world tw, snd tw) \<and> wityping \<Gamma> (snd tw)", rotated 1], rule Assign2, simp)
   using nand_inv_next_time beval_world_raw2_type worldline_upd_preserve_wityping
-  by (metis \<Gamma>.simps(3) eq_snd_iff worldline_upd2_def)
+  by (metis scalar_type_nand3_axioms scalar_type_nand3_def snd_conv worldline_upd2_def)
 
 lemma nand_seq_hoare_next_time0:
   " \<turnstile> [\<lambda>tw. get_time tw = 0 \<and> wityping \<Gamma> (snd tw)] Bassign_trans C (Bnand (Bsig A) (Bsig B)) 1 [\<lambda>tw. nand_inv (next_time_world tw, snd tw) \<and> wityping \<Gamma> (snd tw)]"
@@ -310,7 +346,7 @@ lemma nand_seq_hoare_next_time4:
   " \<turnstile> [\<lambda>tw.  wityping \<Gamma> (snd tw) ] Bassign_trans C (Bnand (Bsig A) (Bsig B)) 1 [\<lambda>tw. nand_inv2 (next_time_world tw, snd tw) \<and> wityping \<Gamma> (snd tw)]"
   apply (rule Conseq2[where Q="\<lambda>tw. nand_inv2 (next_time_world tw, snd tw) \<and> wityping \<Gamma> (snd tw)", rotated 1], rule Assign2, blast)
   using nand_inv2_next_time beval_world_raw2_type
-  by (simp add: worldline_upd_preserve_wityping worldline_upd2_def)
+  by (metis scalar_type_nand3_axioms scalar_type_nand3_def snd_conv worldline_upd2_def worldline_upd_preserve_wityping)
 
 definition "nand_wityping \<equiv> \<lambda>tw. nand_inv tw \<and> wityping \<Gamma> (snd tw)"
 definition "nand_wityping2 \<equiv> \<lambda>tw. nand_inv2 tw \<and> wityping \<Gamma> (snd tw)"
@@ -409,7 +445,7 @@ proof -
     by auto
 qed
 
-subsection \<open>Proving @{term "nand"}: NAND with inertial delay\<close>
+subsubsection \<open>Proving @{term "nand"}: NAND with inertial delay\<close>
 
 lemma nand_inv_next_time_inert:
   assumes "nand_inv tw"
@@ -635,11 +671,12 @@ qed
 lemma nand_seq_hoare_next_time_inert:
   "\<turnstile> [\<lambda>tw. nand_inv tw \<and> wityping \<Gamma> (snd tw)] (Bassign_inert C (Bnand (Bsig A) (Bsig B)) 1) [\<lambda>tw. nand_inv (next_time_world tw, snd tw)]"
   apply (rule Conseq2[where Q="\<lambda>tw. nand_inv (next_time_world tw, snd tw)", rotated 1], rule AssignI2, blast)
-  using nand_inv_next_time_inert beval_world_raw2_type by blast
+  using nand_inv_next_time_inert beval_world_raw2_type
+  using scalar_type_nand3_axioms scalar_type_nand3_def by auto
 
 lemma seq_wt_nand3:
   "seq_wt \<Gamma> (Bassign_inert C (Bnand (Bsig A) (Bsig B)) 1)"
-  by (metis \<Gamma>.elims seq_wt.intros bexp_wt.intros)
+  by (metis bexp_wt.intros(3) bexp_wt.intros(9) scalar_type_nand3_axioms scalar_type_nand3_def seq_wt.intros(5))
 
 lemma nand_seq_hoare_wityping:
   "\<turnstile> [\<lambda>tw. nand_inv tw \<and> wityping \<Gamma> (snd tw)] (Bassign_inert C (Bnand (Bsig A) (Bsig B)) 1) [\<lambda>tw. nand_inv (next_time_world tw, snd tw) \<and> wityping \<Gamma> (snd tw)]"
@@ -653,7 +690,8 @@ lemma nand_seq_hoare_wityping:
 lemma nand_seq_hoare_next_time0_inert:
   " \<turnstile> [\<lambda>tw. get_time tw = 0 \<and> wityping \<Gamma> (snd tw)] Bassign_inert C (Bnand (Bsig A) (Bsig B)) 1 [\<lambda>tw. nand_inv (next_time_world tw, snd tw)]"
   apply (rule Conseq2[where Q="\<lambda>tw. nand_inv (next_time_world tw, snd tw)", rotated 1], rule AssignI2)
-  using nand_inv_next_time0_inert beval_world_raw2_type by auto
+  using nand_inv_next_time0_inert beval_world_raw2_type scalar_type_nand3_axioms scalar_type_nand3_def
+  by auto
 
 lemma nand_seq_hoare_wityping0:
   " \<turnstile> [\<lambda>tw. get_time tw = 0 \<and> wityping \<Gamma> (snd tw)] Bassign_inert C (Bnand (Bsig A) (Bsig B)) 1 [\<lambda>tw. nand_inv (next_time_world tw, snd tw) \<and> wityping \<Gamma> (snd tw)]"
@@ -759,7 +797,8 @@ qed
 lemma nand_seq_hoare_next_time4_inert:
   " \<turnstile> [\<lambda>tw. wityping \<Gamma> (snd tw)] Bassign_inert C (Bnand (Bsig A) (Bsig B)) 1 [\<lambda>tw. nand_inv2 (next_time_world tw, snd tw)]"
   apply (rule Conseq2[where Q="\<lambda>tw. nand_inv2 (next_time_world tw, snd tw)", rotated 1], rule AssignI2, blast)
-  using nand_inv2_next_time_inert beval_world_raw2_type by blast
+  using nand_inv2_next_time_inert beval_world_raw2_type scalar_type_nand3_axioms scalar_type_nand3_def
+  by auto
 
 lemma nand_seq_hoare2_wityping:
   " \<turnstile> [\<lambda>tw. wityping \<Gamma> (snd tw)] Bassign_inert C (Bnand (Bsig A) (Bsig B)) 1 [\<lambda>tw. nand_inv2 (next_time_world tw, snd tw) \<and> wityping \<Gamma> (snd tw)]"
@@ -857,6 +896,967 @@ proof -
   hence "\<forall>i < fst tw'. bval_of_wline tw' C (i + 1) \<longleftrightarrow> \<not> (bval_of_wline tw' A i \<and> bval_of_wline tw' B i)"
     unfolding nand_wityping_def nand_inv_def by auto
   with \<open>i + 1 < fst tw'\<close> show ?thesis
+    by auto
+qed
+
+end
+
+subsection \<open>vector type of NAND\<close>
+
+locale vector_type_nand3 =
+  fixes len :: "nat"
+  fixes \<Gamma> :: "sig tyenv"
+  assumes "\<Gamma> A = Lty len" and "\<Gamma> B = Lty len" and "\<Gamma> C = Lty len"
+begin
+
+definition nand_inv :: "sig assn2" where
+  "nand_inv \<equiv> (\<lambda>tw. \<forall>i < fst tw.
+             lof_wline tw C (i + 1) = map2 (\<lambda>x y. x \<longrightarrow> \<not> y) (lof_wline tw A i) (lof_wline tw B i))"
+
+definition nand_inv2 :: "sig assn2" where
+  "nand_inv2 \<equiv> (\<lambda>tw. disjnt {A, B} (event_of tw) \<longrightarrow>
+             (\<forall>i\<ge>fst tw. lof_wline tw C (i + 1) = map2 (\<lambda>x y. x \<longrightarrow> \<not> y) (lof_wline tw A (fst tw)) (lof_wline tw B (fst tw))))"
+
+lemma nand_inv_next_time:
+  assumes "nand_inv tw"
+  assumes "beval_world_raw2 tw (Bnand (Bsig A) (Bsig B)) v" and "type_of v = Lty len"
+  defines "tw' \<equiv> tw[C, 1 :=\<^sub>2 v]"
+  shows   "nand_inv (next_time_world tw', snd tw')"
+proof -
+  have "fst tw' < next_time_world tw'"
+    using next_time_world_at_least  using nat_less_le by blast
+  moreover have "fst tw = fst tw'"
+    unfolding tw'_def worldline_upd2_def worldline_upd_def by auto
+  ultimately have "fst tw < next_time_world tw'"
+    by auto
+  have "\<forall>i < next_time_world tw'. lof_wline tw' C (i + 1) = map2 (\<lambda>x y. x \<longrightarrow> \<not> y) (lof_wline tw' A i) (lof_wline tw' B i)"
+  proof (rule allI, rule impI)
+    fix i
+    assume "i < next_time_world tw'"
+    hence "i < fst tw \<or> fst tw \<le> i \<and> i < next_time_world tw' - 1 \<or> i = next_time_world tw' - 1"
+      using \<open>fst tw < next_time_world tw'\<close> by linarith
+    moreover
+    { assume "i < fst tw"
+      hence "lof_wline tw C (i + 1) = map2 (\<lambda>x y. x \<longrightarrow> \<not> y) (lof_wline tw A i) (lof_wline tw B i)"
+        using assms(1) unfolding nand_inv_def by auto
+      hence "lof_wline tw' C (i + 1) = map2 (\<lambda>x y. x \<longrightarrow> \<not> y) (lof_wline tw' A i) (lof_wline tw' B i)"
+        unfolding tw'_def worldline_upd2_def worldline_upd_def  by (simp add: \<open>i < get_time tw\<close>) }
+    moreover
+    { assume " fst tw \<le> i \<and> i < next_time_world tw' - 1"
+      hence "lof_wline tw' C (i + 1) = lof_wline tw' C (fst tw + 1)"
+        using unchanged_until_next_time_world
+        by (metis (mono_tags, lifting) Suc_eq_plus1 \<open>get_time tw = get_time tw'\<close> le_Suc_eq le_add1
+        le_less_trans less_diff_conv)
+      moreover have "lof_wline tw' A i = lof_wline tw' A (fst tw)" and "lof_wline tw' B i = lof_wline tw' B (fst tw)"
+        using unchanged_until_next_time_world \<open>fst tw \<le> i \<and> i < next_time_world tw' - 1\<close>
+        by (metis \<open>get_time tw = get_time tw'\<close> \<open>i < next_time_world tw'\<close>)+
+      moreover have "lof_wline tw' C (fst tw + 1) = map2 (\<lambda>x y. x \<longrightarrow> \<not> y) (lof_wline tw' A (fst tw)) (lof_wline tw' B (fst tw))"
+      proof -
+        have assms2: "beval_world_raw (snd tw) (get_time tw) (Bnand (Bsig A) (Bsig B)) v"
+          using assms(2) unfolding beval_world_raw2_def by auto
+        have "wline_of tw' C (fst tw + 1) = v"
+          unfolding tw'_def worldline_upd2_def worldline_upd_def by auto
+        also have "... = Lv (map2 (\<lambda>x y. x \<longrightarrow> \<not> y) (lof_wline tw A (fst tw)) (lof_wline tw B (fst tw)))"
+          apply (rule beval_world_raw_cases[OF assms2], erule beval_cases)
+          prefer 2
+          apply (metis beval_cases(1) comp_def val.sel(2) state_of_world_def)
+          using assms by auto
+        also have "... = Lv (map2 (\<lambda>x y. x \<longrightarrow> \<not> y) (lof_wline tw' A (fst tw)) (lof_wline tw' B (fst tw)))"
+          unfolding tw'_def worldline_upd2_def worldline_upd_def by simp
+        finally show ?thesis
+          by simp
+      qed
+      ultimately have "lof_wline tw' C (i + 1) = map2 (\<lambda>x y. x \<longrightarrow> \<not> y) (lof_wline tw' A i) (lof_wline tw' B i)"
+        by simp }
+    moreover
+    { assume "i = next_time_world tw' - 1"
+      hence "lof_wline tw' C (i + 1) = lof_wline tw' C (next_time_world tw')"
+        using \<open>i < next_time_world tw'\<close> by auto
+      also have "... = lof_wline tw' C (fst tw + 1)"
+        using \<open>fst tw < next_time_world tw'\<close> unfolding tw'_def worldline_upd2_def
+        worldline_upd_def by auto
+      finally have "lof_wline tw' C (i + 1) = lof_wline tw' C (fst tw + 1)"
+        by auto
+      also have "... = map2 (\<lambda>x y. x \<longrightarrow> \<not> y) (lof_wline tw' A (fst tw)) (lof_wline tw' B (fst tw))"
+      proof -
+        have assms2: "beval_world_raw (snd tw) (get_time tw) (Bnand (Bsig A) (Bsig B)) v"
+          using assms(2) unfolding beval_world_raw2_def by auto
+        have "wline_of tw' C (fst tw + 1) = v"
+          unfolding tw'_def worldline_upd2_def worldline_upd_def by auto
+        also have "... = Lv (map2 (\<lambda>x y. x \<longrightarrow> \<not> y)  (lof_wline tw A (fst tw)) (lof_wline tw B (fst tw)))"
+          apply (rule beval_world_raw_cases[OF assms2], erule beval_cases)
+          prefer 2
+          apply (metis beval_cases(1) comp_def val.sel(2) state_of_world_def)
+          using assms by auto
+        also have "... = Lv (map2 (\<lambda>x y. x \<longrightarrow> \<not> y)  (lof_wline tw' A (fst tw)) (lof_wline tw' B (fst tw)))"
+          unfolding tw'_def worldline_upd2_def worldline_upd_def by simp
+        finally show ?thesis
+          by simp
+      qed
+      also have "... = map2 (\<lambda>x y. x \<longrightarrow> \<not> y) (lof_wline tw' A i) (lof_wline tw' B i)"
+        by (metis (no_types, lifting) \<open>get_time tw = get_time tw'\<close> \<open>i < get_time tw \<Longrightarrow> lval_of (wline_of tw' C (i + 1)) = map2 (\<lambda>x y. x \<longrightarrow> \<not> y) (lval_of (wline_of tw' A i)) (lval_of (wline_of tw' B i))\<close> \<open>i < next_time_world tw'\<close> \<open>lval_of (wline_of tw' C (get_time tw + 1)) = map2 (\<lambda>x y. x \<longrightarrow> \<not> y) (lval_of (wline_of tw' A (get_time tw))) (lval_of (wline_of tw' B (get_time tw)))\<close> \<open>lval_of (wline_of tw' C (i + 1)) = lval_of (wline_of tw' C (get_time tw + 1))\<close> le_less_linear unchanged_until_next_time_world)
+      finally have "lof_wline tw' C (i + 1) = map2 (\<lambda>x y. x \<longrightarrow> \<not> y) (lof_wline tw' A i) (lof_wline tw' B i)"
+        by auto }
+    ultimately show "lof_wline tw' C (i + 1) = map2 (\<lambda>x y. x \<longrightarrow> \<not> y) (lof_wline tw' A i) (lof_wline tw' B i)"
+      by auto
+  qed
+  thus ?thesis
+    unfolding nand_inv_def by auto
+qed
+
+lemma nand_seq_hoare_next_time:
+  "\<turnstile> [\<lambda>tw. nand_inv tw \<and> wityping \<Gamma> (snd tw)] (Bassign_trans C (Bnand (Bsig A) (Bsig B)) 1) [\<lambda>tw. nand_inv (next_time_world tw, snd tw) \<and> wityping \<Gamma> (snd tw)]"
+  using nand_inv_next_time beval_world_raw2_type worldline_upd_preserve_wityping
+  by (smt Assign'_hoare2 snd_conv vector_type_nand3_axioms vector_type_nand3_def worldline_upd2_def)
+
+lemma nand_seq_hoare_next_time0:
+  " \<turnstile> [\<lambda>tw. get_time tw = 0 \<and> wityping \<Gamma> (snd tw)] Bassign_trans C (Bnand (Bsig A) (Bsig B)) 1 [\<lambda>tw. nand_inv (next_time_world tw, snd tw) \<and> wityping \<Gamma> (snd tw)]"
+  apply (rule Conseq2[where P="\<lambda>tw. nand_inv tw \<and> wityping \<Gamma> (snd tw)" and Q="\<lambda>tw. nand_inv (next_time_world tw, snd tw) \<and> wityping \<Gamma> (snd tw)"])
+  using nand_seq_hoare_next_time unfolding nand_inv_def  using gr_implies_not_zero
+  by auto
+
+lemma nand_conc_hoare':
+  "\<And>tw. nand_inv tw \<and> nand_inv2 tw \<and> disjnt {A, B} (event_of tw) \<Longrightarrow> nand_inv (next_time_world tw, snd tw)"
+proof -
+  fix tw
+  assume "nand_inv tw \<and> nand_inv2 tw \<and> disjnt {A, B} (event_of tw)"
+  hence "nand_inv tw" and "nand_inv2 tw" and "disjnt {A, B} (event_of tw)"
+    by auto
+  hence *: "\<forall>i < fst tw. lof_wline tw C (i + 1) = map2 (\<lambda>x y. x \<longrightarrow> \<not> y) (lof_wline tw A i) (lof_wline tw B i)"
+    unfolding nand_inv_def by auto
+  have **: "\<forall>i\<ge>fst tw. i < next_time_world tw \<longrightarrow> (\<forall>s. lof_wline tw s i = lof_wline tw s (fst tw))"
+    using unchanged_until_next_time_world by metis
+  have ***: "(\<forall>i\<ge> fst tw. lof_wline tw C (i + 1) = map2 (\<lambda>x y. x \<longrightarrow> \<not> y) (lof_wline tw A (fst tw)) (lof_wline tw B (fst tw)))"
+    using \<open>nand_inv2 tw\<close> \<open>disjnt {A, B} (event_of tw)\<close> unfolding nand_inv2_def by auto
+
+  \<comment> \<open>obtain the value of A and B at time fst tw\<close>
+  have "lof_wline tw A (fst tw) = lof_wline tw A (fst tw - 1)" and
+        "lof_wline tw B (fst tw) = lof_wline tw B (fst tw - 1)"
+    using \<open>disjnt {A, B} (event_of tw)\<close> unfolding event_of_alt_def
+    by (smt diff_0_eq_0 disjnt_insert1 mem_Collect_eq)+
+ { fix i
+    assume "i < next_time_world tw"
+    have "i < fst tw \<or> fst tw \<le> i"
+      by auto
+    moreover
+    { assume "i < fst tw"
+      hence "lof_wline tw C (i + 1) = map2 (\<lambda>x y. x \<longrightarrow> \<not> y) (lof_wline tw A i) (lof_wline tw B i)"
+        using * by auto }
+    moreover
+    { assume "fst tw \<le> i"
+      hence "lof_wline tw C (i + 1) = lof_wline tw C (fst tw + 1)"
+        using *** by auto
+      also have "... = map2 (\<lambda>x y. x \<longrightarrow> \<not> y) (lof_wline tw A (fst tw)) (lof_wline tw B (fst tw))"
+        using *** \<open>fst tw \<le> i\<close> by auto
+      also have "... = map2 (\<lambda>x y. x \<longrightarrow> \<not> y) (lof_wline tw A i) (lof_wline tw B i)"
+        using ** \<open>fst tw \<le> i\<close> less_imp_le_nat  by (simp add: \<open>i < next_time_world tw\<close>)
+      finally have "lof_wline tw C (i + 1) = map2 (\<lambda>x y. x \<longrightarrow> \<not> y) (lof_wline tw A i) (lof_wline tw B i)"
+        by auto }
+    ultimately have "lof_wline tw C (i + 1) = map2 (\<lambda>x y. x \<longrightarrow> \<not> y) (lof_wline tw A i) (lof_wline tw B i)"
+      by auto }
+  hence "\<And>i. i < next_time_world tw \<Longrightarrow> lof_wline tw C (i + 1) = map2 (\<lambda>x y. x \<longrightarrow> \<not> y) (lof_wline tw A i) (lof_wline tw B i)"
+    by auto
+  thus "nand_inv (next_time_world tw, snd tw)"
+    unfolding nand_inv_def by auto
+qed
+
+lemma nand_conc_hoare2:
+  "\<And>tw. nand_inv tw \<and> nand_inv2 tw \<and> disjnt {A, B} (event_of tw) \<Longrightarrow> nand_inv2 (next_time_world tw, snd tw)"
+proof -
+  fix tw
+  assume "nand_inv tw \<and> nand_inv2 tw \<and> disjnt {A, B} (event_of tw)"
+  hence "nand_inv tw" and "nand_inv2 tw" and "disjnt {A, B} (event_of tw)"
+    by auto
+  hence 0: "\<forall>i \<ge> fst tw. lof_wline tw C (i + 1) = map2 (\<lambda>x y. x \<longrightarrow> \<not> y) (lof_wline tw A (fst tw)) (lof_wline tw B (fst tw))"
+    unfolding nand_inv2_def by auto
+  have 1: "\<forall>i\<ge>fst tw. i < next_time_world tw \<longrightarrow> (\<forall>s. lof_wline tw s i = lof_wline tw s (fst tw))"
+    using unchanged_until_next_time_world by metis
+  let ?t' = "next_time_world tw"
+  { assume "disjnt {A, B} (event_of (next_time_world tw, snd tw))"
+    hence *: "lof_wline tw A ?t' = lof_wline tw A (?t' - 1)" and **: "lof_wline tw B ?t' = lof_wline tw B (?t' - 1)"
+      unfolding event_of_alt_def
+      by (smt comp_apply diff_0_eq_0 disjnt_insert1 fst_conv mem_Collect_eq snd_conv)+
+    have "fst tw < next_time_world tw"
+      by (simp add: next_time_world_at_least)
+    { fix i
+      assume "?t' \<le> i"
+      hence "lof_wline tw C (i + 1) = map2 (\<lambda>x y. x \<longrightarrow> \<not> y) (lof_wline tw A (fst tw)) (lof_wline tw B (fst tw))"
+        using 0 \<open>fst tw < ?t'\<close> by auto
+      moreover have "lof_wline tw A (fst tw) = lof_wline tw A (?t' - 1)" and "lof_wline tw B (fst tw) = lof_wline tw B (?t' - 1)"
+        using 1
+        by (metis (no_types, lifting) One_nat_def Suc_leI \<open>get_time tw < next_time_world tw\<close>
+        add_le_cancel_right diff_add diff_less discrete gr_implies_not_zero neq0_conv zero_less_one)+
+      ultimately have "lof_wline tw C (i + 1) = map2 (\<lambda>x y. x \<longrightarrow> \<not> y) (lof_wline tw A ?t') (lof_wline tw B ?t')"
+        using * ** by auto }
+    hence "(\<forall>i\<ge>?t'. lof_wline tw C (i + 1) = map2 (\<lambda>x y. x \<longrightarrow> \<not> y) (lof_wline tw A ?t') (lof_wline tw B ?t'))"
+      by auto }
+  thus "nand_inv2 (next_time_world tw, snd tw)"
+    unfolding nand_inv2_def by auto
+qed
+
+lemma nand_inv2_next_time:
+  fixes tw
+  assumes "beval_world_raw2 tw (Bnand (Bsig A) (Bsig B)) v" and "type_of v = Lty len"
+  defines "tw' \<equiv> tw[C, 1 :=\<^sub>2 v]"
+  shows   "nand_inv2 (next_time_world tw', snd tw')"
+proof -
+  { assume "disjnt {A, B} (event_of (next_time_world tw', snd tw'))"
+    let ?t' = "next_time_world tw'"
+    have "fst tw' < ?t'"
+      using next_time_world_at_least by blast
+    moreover have "fst tw = fst tw'"
+      unfolding tw'_def unfolding worldline_upd2_def by auto
+    ultimately have "fst tw < ?t'"
+      by auto
+    have *: "\<And>s. s \<in> {A, B} \<Longrightarrow> lof_wline tw' s ?t' = lof_wline tw s (fst tw)"
+    proof -
+      fix s
+      assume "s \<in> {A, B}"
+      hence "lof_wline tw' s ?t' = lof_wline tw s ?t'"
+        unfolding tw'_def worldline_upd2_def worldline_upd_def by auto
+      also have "... = lof_wline tw s (?t' - 1)"
+        using \<open>disjnt {A, B} (event_of (next_time_world tw', snd tw'))\<close> \<open>fst tw < ?t'\<close>
+        unfolding event_of_alt_def
+        by (smt \<open>s \<in> {A, B}\<close> comp_apply disjnt_iff fst_conv gr_implies_not_zero insert_iff
+        mem_Collect_eq sig.simps(4) sig.simps(6) singletonD snd_conv tw'_def worldline_upd2_def
+        worldline_upd_def)
+      also have "... = lof_wline tw s (fst tw)"
+      proof -
+        have "fst tw' \<le> ?t' - 1" and "?t' - 1 < ?t'"
+          using \<open>fst tw' < ?t'\<close> by auto
+        hence "lof_wline tw' s (?t' - 1) = lof_wline tw' s (fst tw')"
+          using unchanged_until_next_time_world[where tw="tw'"] by metis
+        moreover have "lof_wline tw' s (?t' - 1) = lof_wline tw s (?t' - 1)"
+          unfolding tw'_def worldline_upd2_def worldline_upd_def using  \<open>s \<in> {A, B}\<close> by auto
+        moreover have "lof_wline tw' s (fst tw') = lof_wline tw s (fst tw')"
+          unfolding tw'_def worldline_upd2_def worldline_upd_def by auto
+        ultimately show ?thesis
+          using \<open>fst tw = fst tw'\<close> by auto
+      qed
+      finally show "lof_wline tw' s ?t' = lof_wline tw s (fst tw)"
+        by auto
+    qed
+    have "\<And>i. ?t' \<le> i \<Longrightarrow> lof_wline tw' C (i + 1) = map2 (\<lambda>x y. x \<longrightarrow> \<not> y) (lof_wline tw' A ?t') (lof_wline tw' B ?t')"
+    proof -
+      fix i
+      have assms2: "beval_world_raw (snd tw) (fst tw) (Bnand (Bsig A) (Bsig B)) v"
+        using assms unfolding beval_world_raw2_def by auto
+      assume "?t' \<le> i"
+      hence "lof_wline tw' C (i + 1) = lval_of v"
+        using `fst tw < ?t'`
+        unfolding tw'_def worldline_upd2_def worldline_upd_def by auto
+      also have "... = map2 (\<lambda>x y. x \<longrightarrow> \<not> y) (lof_wline tw A (fst tw)) (lof_wline tw B (fst tw))"
+        apply (rule beval_world_raw_cases[OF assms2], erule beval_cases)
+        prefer 2
+        apply (metis beval_cases(1) comp_def state_of_world_def val.sel(2))
+        using assms(2) by auto
+      also have "... = map2 (\<lambda>x y. x \<longrightarrow> \<not> y) (lof_wline tw' A ?t') (lof_wline tw' B ?t')"
+        using * by auto
+      finally show "lof_wline tw' C (i + 1) = map2 (\<lambda>x y. x \<longrightarrow> \<not> y) (lof_wline tw' A ?t') (lof_wline tw' B ?t')"
+        by auto
+    qed }
+  thus ?thesis
+    unfolding nand_inv2_def by auto
+qed
+
+lemma nand_seq_hoare_next_time4:
+  " \<turnstile> [\<lambda>tw.  wityping \<Gamma> (snd tw) ] Bassign_trans C (Bnand (Bsig A) (Bsig B)) 1 [\<lambda>tw. nand_inv2 (next_time_world tw, snd tw) \<and> wityping \<Gamma> (snd tw)]"
+  apply (rule Conseq2[where Q="\<lambda>tw. nand_inv2 (next_time_world tw, snd tw) \<and> wityping \<Gamma> (snd tw)", rotated 1], rule Assign2, blast)
+  using nand_inv2_next_time beval_world_raw2_type
+  by (metis snd_conv vector_type_nand3_axioms vector_type_nand3_def worldline_upd2_def worldline_upd_preserve_wityping)
+
+lemma nand_conc_hoare3_without:
+  "\<turnstile> \<lbrace>\<lambda>tw. (nand_inv tw \<and> wityping \<Gamma> (snd tw)) \<and> nand_inv2 tw\<rbrace>
+        nand3
+     \<lbrace>\<lambda>tw. nand_inv (next_time_world tw, snd tw)  \<and> nand_inv2  (next_time_world tw, snd tw)\<rbrace>"
+  unfolding nand3_def
+  apply (rule Single)
+   apply (rule Conj)
+    apply (rule strengthen_precondition)
+    apply (rule strengthen_precondition)
+  apply (rule weaken_postcondition[OF nand_seq_hoare_next_time])
+   apply (rule strengthen_precondition)
+   apply (rule strengthen_precondition)
+   apply (rule strengthen_precondition2)
+  apply (rule weaken_postcondition[OF nand_seq_hoare_next_time4])
+  apply (rule, rule)
+  using nand_conc_hoare' nand_conc_hoare2 by blast
+
+lemma nand3_conc_wt:
+  " conc_wt \<Gamma> ( process {A, B} : Bassign_trans C (Bnand (Bsig A) (Bsig B)) 1)"
+  apply (intro conc_wt.intros)
+  apply (intro seq_wt.intros)
+  apply (intro bexp_wt.intros)
+  by (metis bexp_wt.intros(3) vector_type_nand3_axioms vector_type_nand3_def)+
+
+lemma nand3_seq_wt:
+  "seq_wt \<Gamma> (Bassign_trans C (Bnand (Bsig A) (Bsig B)) 1)"
+  using nand3_conc_wt by blast
+
+lemma nand_conc_hoare3:
+  "\<turnstile> \<lbrace>\<lambda>tw. (nand_inv tw \<and> wityping \<Gamma> (snd tw)) \<and> nand_inv2 tw\<rbrace>
+        nand3
+     \<lbrace>\<lambda>tw. (nand_inv (next_time_world tw, snd tw)  \<and> nand_inv2  (next_time_world tw, snd tw)) \<and> wityping \<Gamma> (snd tw)\<rbrace>"
+  apply (rule Conj2)
+   apply (rule nand_conc_hoare3_without)
+  apply (rule strengthen_pre_conc_hoare)
+   prefer 2
+  unfolding nand3_def apply (rule single_conc_stmt_preserve_wityping_hoare)
+   apply (rule nand3_seq_wt)
+  apply blast
+  done
+
+lemma nand_conc_sim':
+  "\<turnstile>\<^sub>s \<lbrace>\<lambda>tw. (nand_inv tw \<and> wityping \<Gamma> (snd tw)) \<and> nand_inv2 tw\<rbrace> nand3 \<lbrace>\<lambda>tw. (nand_inv tw \<and> wityping \<Gamma> (snd tw)) \<and> nand_inv2 tw\<rbrace>"
+  apply (rule While)
+  apply (rule Conseq')
+    prefer 2
+    apply (rule nand_conc_hoare3)
+   apply blast
+  unfolding snd_conv apply blast
+  done
+
+lemma nand_conc_sim2':
+  "\<turnstile>\<^sub>s \<lbrace>\<lambda>tw. (nand_inv tw \<and> wityping \<Gamma> (snd tw)) \<and> nand_inv2 tw\<rbrace> nand3 \<lbrace>\<lambda>tw. nand_inv tw \<and> wityping \<Gamma> (snd tw)\<rbrace>"
+  apply (rule Conseq_sim[rotated])
+  by (rule nand_conc_sim') blast+
+
+lemma init_sat_nand_inv:
+  "init_sim_hoare (\<lambda>tw. fst tw = 0 \<and> wityping \<Gamma> (snd tw)) nand3 (\<lambda>tw. nand_inv tw \<and> wityping \<Gamma> (snd tw))"
+  unfolding nand3_def
+  apply (rule AssignI)
+  apply (rule SingleI)
+  unfolding snd_conv
+  apply (rule nand_seq_hoare_next_time0)
+  done
+
+lemma init_sat_nand_inv2:
+  "init_sim_hoare (\<lambda>tw. wityping \<Gamma> (snd tw)) nand3 (\<lambda>tw. nand_inv2 tw \<and> wityping \<Gamma> (snd tw))"
+  unfolding nand3_def
+  apply (rule AssignI)
+  apply (rule SingleI)
+  unfolding snd_conv
+  apply (rule nand_seq_hoare_next_time4)
+  done
+
+lemma init_sat_nand_inv_comb:
+  "init_sim_hoare (\<lambda>tw. fst tw = 0 \<and> wityping \<Gamma> (snd tw)) nand3 (\<lambda>tw. (nand_inv tw \<and>  wityping \<Gamma> (snd tw)) \<and> nand_inv2 tw)"
+  apply (rule ConjI_sim)
+  apply (rule init_sat_nand_inv)
+  apply (rule ConseqI_sim[rotated])
+    apply (rule init_sat_nand_inv2)
+   apply simp
+  apply simp
+  done
+
+lemma nand_correctness:
+  assumes "sim_fin w (i + 1) nand3 tw'" and "wityping \<Gamma> w"
+  shows "lof_wline tw' C (i + 1) = map2 (\<lambda>x y. x \<longrightarrow> \<not> y) (lof_wline tw' A i)  (lof_wline tw' B i)"
+proof -
+  obtain tw where "init_sim (0, w) nand3 tw" and  "tw, i + 1, nand3 \<Rightarrow>\<^sub>S tw'"
+    using premises_sim_fin_obt[OF assms(1)] by auto
+  hence "i + 1 < fst tw'"
+    using world_maxtime_lt_fst_tres  by blast
+  have "conc_stmt_wf nand3"
+    unfolding conc_stmt_wf_def nand3_def by auto
+  moreover have "nonneg_delay_conc nand3"
+    unfolding nand3_def by auto
+  ultimately have "init_sim_valid (\<lambda>tw. fst tw = 0 \<and> wityping \<Gamma> (snd tw)) nand3 (\<lambda>tw. (nand_inv tw \<and> wityping \<Gamma> (snd tw)) \<and> nand_inv2 tw)"
+    using init_sim_hoare_soundness[OF init_sat_nand_inv_comb] by auto
+  hence "(nand_inv tw \<and> wityping \<Gamma> (snd tw)) \<and> nand_inv2 tw"
+    using \<open>init_sim (0, w) nand3 tw\<close> fst_conv assms(2) unfolding init_sim_valid_def
+    by (metis snd_conv)
+  hence "nand_inv tw \<and> wityping \<Gamma> (snd tw)" and "nand_inv2 tw"
+    by auto
+  moreover have "\<Turnstile>\<^sub>s \<lbrace>\<lambda>tw. (nand_inv tw \<and> wityping \<Gamma> (snd tw)) \<and> nand_inv2 tw\<rbrace> nand3 \<lbrace>\<lambda>tw. nand_inv tw \<and> wityping \<Gamma> (snd tw)\<rbrace>"
+    using conc_sim_soundness[OF nand_conc_sim2'] \<open>conc_stmt_wf nand3\<close> \<open>nonneg_delay_conc nand3\<close>
+    by auto
+  ultimately have "nand_inv tw' \<and> wityping \<Gamma> (snd tw)"
+    using \<open>tw, i + 1, nand3 \<Rightarrow>\<^sub>S tw'\<close> unfolding sim_hoare_valid_def by blast
+  hence "\<forall>i < fst tw'. lof_wline tw' C (i + 1) = map2 (\<lambda>x y. x \<longrightarrow> \<not> y) (lof_wline tw' A i) (lof_wline tw' B i)"
+    unfolding nand_inv_def by auto
+  with \<open>i + 1 < fst tw'\<close> show ?thesis
+    by auto
+qed
+
+lemma nand_inv_next_time_inert:
+  assumes "nand_inv tw"
+  assumes "beval_world_raw2 tw (Bnand (Bsig A) (Bsig B)) v" and "type_of v = Lty len"
+  defines "tw' \<equiv> tw\<lbrakk>C, 1 :=\<^sub>2 v\<rbrakk>"
+  shows   "nand_inv (next_time_world tw', snd tw')"
+proof -
+  have "fst tw' < next_time_world tw'"
+    using next_time_world_at_least  using nat_less_le by blast
+  moreover have "fst tw = fst tw'"
+    unfolding tw'_def worldline_inert_upd2_def by auto
+  ultimately have "fst tw < next_time_world tw'"
+    by auto
+  have "\<forall>i < next_time_world tw'. lof_wline tw' C (i + 1) = map2 (\<lambda>x y. x \<longrightarrow> \<not> y) (lof_wline tw' A i) (lof_wline tw' B i)"
+  proof (rule allI, rule impI)
+    fix i
+    assume "i < next_time_world tw'"
+    hence "i < fst tw \<or> fst tw \<le> i \<and> i < next_time_world tw' - 1 \<or> i = next_time_world tw' - 1"
+      using \<open>fst tw < next_time_world tw'\<close> by linarith
+    moreover
+    { assume "i < fst tw"
+      hence "lof_wline tw C (i + 1) = map2 (\<lambda>x y. x \<longrightarrow> \<not> y) (lof_wline tw A i) (lof_wline tw B i)"
+        using assms(1) unfolding nand_inv_def by auto
+      have "lof_wline tw' C (i + 1) = map2 (\<lambda>x y. x \<longrightarrow> \<not> y) (lof_wline tw' A i) (lof_wline tw' B i)"
+      proof (cases "i + 1 < fst tw")
+        case True
+        hence "lof_wline tw' C (i + 1) = lof_wline tw C (i + 1)"
+          unfolding tw'_def worldline_inert_upd2_def worldline_inert_upd_def Let_def
+          by auto
+        also have "... = map2 (\<lambda>x y. x \<longrightarrow> \<not> y) (lof_wline tw A i) (lof_wline tw B i)"
+          using `lof_wline tw C (i + 1) = map2 (\<lambda>x y. x \<longrightarrow> \<not> y) (lof_wline tw A i) (lof_wline tw B i)`
+          by auto
+        also have "... = map2 (\<lambda>x y. x \<longrightarrow> \<not> y) (lof_wline tw' A i) (lof_wline tw' B i)"
+          unfolding tw'_def worldline_inert_upd2_def worldline_inert_upd_def Let_def
+          by auto
+        finally show ?thesis
+          by auto
+      next
+        case False
+        hence "i + 1 = fst tw"
+          using \<open>i < get_time tw\<close> by linarith
+        show "lof_wline tw' C (i + 1) = map2 (\<lambda>x y. x \<longrightarrow> \<not> y) (lof_wline tw' A i) (lof_wline tw' B i)"
+        proof (cases "wline_of tw C (get_time tw) = v \<or> wline_of tw C (get_time tw + 1) \<noteq> v")
+          case True
+          hence "lof_wline tw' C (i + 1) = lof_wline tw C (fst tw)"
+            using `i + 1 = fst tw`
+            unfolding tw'_def worldline_inert_upd2_def worldline_inert_upd_def by auto
+          also have "... = map2 (\<lambda>x y. x \<longrightarrow> \<not> y) (lof_wline tw A i) (lof_wline tw B i)"
+            using `lof_wline tw C (i + 1) = map2 (\<lambda>x y. x \<longrightarrow> \<not> y) (lof_wline tw A i) (lof_wline tw B i)`
+            `i + 1 = fst tw` by auto
+          also have "... = map2 (\<lambda>x y. x \<longrightarrow> \<not> y) (lof_wline tw' A i) (lof_wline tw' B i)"
+            unfolding tw'_def worldline_inert_upd2_def worldline_inert_upd_def Let_def
+            using `i + 1 = fst tw` by auto
+          finally show ?thesis
+            by auto
+        next
+          case False
+          hence "wline_of tw C (fst tw) \<noteq> v" and "wline_of tw C (fst tw + 1) = v"
+            by auto
+          let ?time = "GREATEST n. n \<le> fst tw + 1
+                                 \<and> wline_of tw C (n - 1) \<noteq> v
+                                 \<and> wline_of tw C n = v"
+          have "?time = fst tw + 1"
+            using False by (intro Greatest_equality) auto
+          hence "wline_of tw' C (i + 1) = wline_of tw C (fst tw)"
+            using False \<open>i + 1 = get_time tw\<close> unfolding tw'_def worldline_inert_upd2_def
+            worldline_inert_upd_def comp_def by auto
+          have "lof_wline tw C (fst tw) = map2 (\<lambda>x y. x \<longrightarrow> \<not> y) (lof_wline tw A i) (lof_wline tw B i)"
+            using `lof_wline tw C (i + 1) = map2 (\<lambda>x y. x \<longrightarrow> \<not> y) (lof_wline tw A i) (lof_wline tw B i)` `i
+            + 1 = fst tw` by auto
+          also have "... = map2 (\<lambda>x y. x \<longrightarrow> \<not> y) (lof_wline tw' A i) (lof_wline tw' B i)"
+            unfolding tw'_def worldline_inert_upd2_def worldline_inert_upd_def Let_def
+            using `i + 1 = fst tw` by auto
+          finally show ?thesis
+            using \<open>wline_of tw' C (i + 1) = wline_of tw C (get_time tw)\<close> by auto
+        qed
+      qed }
+    moreover
+    { assume " fst tw \<le> i \<and> i < next_time_world tw' - 1"
+      hence "lof_wline tw' C (i + 1) = lof_wline tw' C (fst tw + 1)"
+        using unchanged_until_next_time_world
+        by (metis (mono_tags, lifting) Suc_eq_plus1 \<open>get_time tw = get_time tw'\<close> le_Suc_eq le_add1
+        le_less_trans less_diff_conv)
+      moreover have "lof_wline tw' A i = lof_wline tw' A (fst tw)" and "lof_wline tw' B i = lof_wline tw' B (fst tw)"
+        by (metis \<open>get_time tw = get_time tw'\<close> \<open>get_time tw \<le> i \<and> i < next_time_world tw' - 1\<close> \<open>i <
+        next_time_world tw'\<close> unchanged_until_next_time_world)+
+      moreover have "lof_wline tw' C (fst tw + 1) = map2 (\<lambda>x y. x \<longrightarrow> \<not> y) (lof_wline tw' A (fst tw)) (lof_wline tw' B (fst tw))"
+      proof (cases " wline_of tw C (get_time tw) = v \<or>  wline_of tw C (get_time tw + 1) \<noteq> v")
+        case True
+        hence "wline_of tw' C (fst tw + 1) = v"
+          unfolding tw'_def worldline_inert_upd2_def worldline_inert_upd_def Let_def by auto
+        have assms2: "beval_world_raw (snd tw) (fst tw) (Bnand (Bsig A) (Bsig B)) v"
+          using \<open>beval_world_raw2 tw (Bnand (Bsig A) (Bsig B)) v\<close> unfolding beval_world_raw2_def
+          by auto
+        have "lval_of v = map2 (\<lambda>x y. x \<longrightarrow> \<not> y) (lof_wline tw A (fst tw)) (lof_wline tw B (fst tw))"
+          apply (rule beval_world_raw_cases[OF assms2], erule beval_cases)
+          prefer 2
+          apply (metis beval_cases(1) comp_def state_of_world_def val.sel(2))
+          using assms(3) by auto
+        also have "... = map2 (\<lambda>x y. x \<longrightarrow> \<not> y) (lof_wline tw' A (fst tw)) (lof_wline tw' B (fst tw))"
+          unfolding tw'_def worldline_inert_upd2_def worldline_inert_upd_def Let_def by auto
+        finally show ?thesis
+          using \<open>wline_of tw' C (get_time tw + 1) = v\<close> by blast
+      next
+        case False
+        hence "wline_of tw C (get_time tw) \<noteq> v" and
+              "wline_of tw C (get_time tw + 1) = v"
+          by blast+
+        let ?time = "GREATEST n. n \<le> get_time tw + 1  \<and> wline_of tw C (n - 1) \<noteq> v  \<and> wline_of tw C n = v"
+        have "?time = fst tw + 1"
+          using False
+          by (intro Greatest_equality) auto
+        hence "wline_of tw' C (fst tw + 1) =  v"
+          using False unfolding tw'_def worldline_inert_upd2_def worldline_inert_upd_def Let_def
+          comp_def by auto
+        have assms2: "beval_world_raw (snd tw) (fst tw) (Bnand (Bsig A) (Bsig B)) v"
+          using \<open>beval_world_raw2 tw (Bnand (Bsig A) (Bsig B)) v\<close> unfolding beval_world_raw2_def
+          by auto
+        have "lval_of v = map2 (\<lambda>x y. x \<longrightarrow> \<not> y) (lof_wline tw A (fst tw)) (lof_wline tw B (fst tw))"
+          unfolding beval_world_raw2_def
+          apply (rule beval_world_raw_cases[OF assms2], erule beval_cases)
+          prefer 2
+          apply (metis beval_cases(1) comp_def state_of_world_def val.sel(2))
+          using assms(3) by auto
+        also have "... = map2 (\<lambda>x y. x \<longrightarrow> \<not> y) (lof_wline tw' A (fst tw)) (lof_wline tw' B (fst tw))"
+          unfolding tw'_def worldline_inert_upd2_def worldline_inert_upd_def Let_def by auto
+        finally show ?thesis
+          using \<open>wline_of tw' C (get_time tw + 1) = v\<close> by auto
+      qed
+      ultimately have "lof_wline tw' C (i + 1) = map2 (\<lambda>x y. x \<longrightarrow> \<not> y) (lof_wline tw' A i) (lof_wline tw' B i)"
+        by auto }
+    moreover
+    { assume "i = next_time_world tw' - 1"
+      hence "lof_wline tw' C (i + 1) = lof_wline tw' C (next_time_world tw')"
+        using \<open>i < next_time_world tw'\<close> by auto
+      also have "... = lof_wline tw' C (fst tw + 1)"
+      proof (cases "wline_of tw C (get_time tw) =  v \<or> wline_of tw C (get_time tw + 1) \<noteq>  v")
+        case True
+        hence "wline_of tw' C (next_time_world tw') = v"
+          unfolding tw'_def worldline_inert_upd2_def worldline_inert_upd_def comp_def
+          using `fst tw < next_time_world tw'`
+          by (smt add.commute fst_conv less_SucE next_time_world_at_least order.asym plus_1_eq_Suc
+          snd_conv)
+        also have "... = wline_of tw' C (fst tw + 1)"
+          by (smt True dual_order.strict_iff_order not_add_less1 o_apply snd_conv tw'_def
+          worldline_inert_upd2_def worldline_inert_upd_def)
+        finally show ?thesis
+          by auto
+      next
+        case False
+        let ?time = "GREATEST n. n \<le> get_time tw + 1  \<and> wline_of tw C (n - 1) \<noteq> v  \<and> wline_of tw C n = v"
+        have "?time = fst tw + 1"
+          using False by (intro Greatest_equality) auto
+        hence "wline_of tw' C (next_time_world tw') = v"
+          unfolding tw'_def worldline_inert_upd2_def worldline_inert_upd_def comp_def
+          by (smt add.commute fst_conv less_SucE next_time_world_at_least order.asym plus_1_eq_Suc
+          snd_conv)
+        also have "... = wline_of tw' C (fst tw + 1)"
+          unfolding tw'_def worldline_inert_upd2_def worldline_inert_upd_def comp_def
+          using `fst tw < next_time_world tw'` `?time = fst tw + 1` by auto
+        finally show ?thesis
+          by auto
+      qed
+      finally have "lof_wline tw' C (i + 1) = lof_wline tw' C (fst tw + 1)"
+        by auto
+      also have "... = map2 (\<lambda>x y. x \<longrightarrow> \<not> y) (lof_wline tw' A (fst tw)) (lof_wline tw' B (fst tw))"
+      proof (cases "wline_of tw C (get_time tw) = v \<or> wline_of tw C (get_time tw + 1) \<noteq> v")
+        case True
+        hence "wline_of tw' C (fst tw + 1) = v"
+          unfolding tw'_def worldline_inert_upd2_def worldline_inert_upd_def Let_def comp_def
+          by auto
+        have assms2: "beval_world_raw (snd tw) (fst tw) (Bnand (Bsig A) (Bsig B)) v"
+          using \<open>beval_world_raw2 tw (Bnand (Bsig A) (Bsig B)) v\<close> unfolding beval_world_raw2_def
+          by auto
+        have "lval_of ... = map2 (\<lambda>x y. x \<longrightarrow> \<not> y) (lof_wline tw A (fst tw)) (lof_wline tw B (fst tw))"
+          apply (rule beval_world_raw_cases[OF assms2], erule beval_cases)
+           prefer 2
+          apply (metis beval_cases(1) comp_def state_of_world_def val.sel(2))
+          using assms(3) by auto
+        also have "... = map2 (\<lambda>x y. x \<longrightarrow> \<not> y) (lof_wline tw' A (fst tw)) (lof_wline tw' B (fst tw))"
+          unfolding tw'_def worldline_inert_upd2_def worldline_inert_upd_def Let_def by auto
+        finally show ?thesis
+          using \<open>wline_of tw' C (get_time tw + 1) = v\<close> by auto
+      next
+        case False
+        let ?time = "GREATEST n. n \<le> get_time tw + 1  \<and> wline_of tw C (n - 1) \<noteq> v  \<and> wline_of tw C n = v"
+        have "?time = fst tw + 1"
+          using False by (intro Greatest_equality) auto
+        hence "wline_of tw' C (fst tw + 1) =  v"
+          unfolding tw'_def worldline_inert_upd2_def worldline_inert_upd_def Let_def comp_def by auto
+        have assms2: "beval_world_raw (snd tw) (fst tw) (Bnand (Bsig A) (Bsig B)) v"
+          using \<open>beval_world_raw2 tw (Bnand (Bsig A) (Bsig B)) v\<close> unfolding beval_world_raw2_def
+          by auto
+        have "lval_of ... = map2 (\<lambda>x y. x \<longrightarrow> \<not> y) (lof_wline tw A (fst tw)) (lof_wline tw B (fst tw))"
+          apply (rule beval_world_raw_cases[OF assms2], erule beval_cases)
+          prefer 2
+          apply (metis beval_cases(1) comp_apply state_of_world_def val.sel(2))
+          using assms(3) by auto
+        also have "... = map2 (\<lambda>x y. x \<longrightarrow> \<not> y) (lof_wline tw' A (fst tw)) (lof_wline tw' B (fst tw))"
+          unfolding tw'_def worldline_inert_upd2_def worldline_inert_upd_def Let_def by auto
+        finally show ?thesis
+          using \<open>wline_of tw' C (get_time tw + 1) = v\<close> by blast
+      qed
+      also have "... = map2 (\<lambda>x y. x \<longrightarrow> \<not> y) (lof_wline tw' A i) (lof_wline tw' B i)"
+        by (metis (no_types, lifting) \<open>get_time tw = get_time tw'\<close> \<open>i < get_time tw \<Longrightarrow> lof_wline tw'
+        C (i + 1) = map2 (\<lambda>x y. x \<longrightarrow> \<not> y) (lof_wline tw' A i) (lof_wline tw' B i)\<close> \<open>i <
+        next_time_world tw'\<close> \<open>lof_wline tw' C (get_time tw + 1) = map2 (\<lambda>x y. x \<longrightarrow> \<not> y) (lof_wline
+        tw' A (get_time tw)) (lof_wline tw' B (get_time tw))\<close> \<open>lof_wline tw' C (i + 1) = lof_wline
+        tw' C (get_time tw + 1)\<close> le_less_linear unchanged_until_next_time_world)
+      finally have "lof_wline tw' C (i + 1) = map2 (\<lambda>x y. x \<longrightarrow> \<not> y) (lof_wline tw' A i) (lof_wline tw' B i)"
+        by auto }
+    ultimately show "lof_wline tw' C (i + 1) = map2 (\<lambda>x y. x \<longrightarrow> \<not> y) (lof_wline tw' A i) (lof_wline tw' B i)"
+      by auto
+  qed
+  thus ?thesis
+    unfolding nand_inv_def by auto
+qed
+
+lemma nand_inv_next_time0_inert:
+  assumes "fst tw = 0"
+  assumes "beval_world_raw2 tw (Bnand (Bsig A) (Bsig B)) v" and "type_of v = Lty len"
+  defines "tw' \<equiv> tw\<lbrakk>C, 1 :=\<^sub>2 v\<rbrakk>"
+  shows   "nand_inv (next_time_world tw', snd tw')"
+proof -
+  have "nand_inv tw"
+    using assms(1) unfolding nand_inv_def by auto
+  from nand_inv_next_time_inert[OF this] show ?thesis
+    unfolding tw'_def using assms by blast
+qed
+
+lemma nand_seq_hoare_next_time_inert:
+  "\<turnstile> [\<lambda>tw. nand_inv tw \<and> wityping \<Gamma> (snd tw)] (Bassign_inert C (Bnand (Bsig A) (Bsig B)) 1) [\<lambda>tw. nand_inv (next_time_world tw, snd tw)]"
+  apply (rule Conseq2[where Q="\<lambda>tw. nand_inv (next_time_world tw, snd tw)", rotated 1], rule AssignI2, blast)
+  using nand_inv_next_time_inert beval_world_raw2_type
+  using vector_type_nand3_axioms vector_type_nand3_def by auto
+
+lemma seq_wt_nand3:
+  "seq_wt \<Gamma> (Bassign_inert C (Bnand (Bsig A) (Bsig B)) 1)"
+  by (metis bexp_wt.intros(3) bexp_wt.intros(9) seq_wt.intros(5) vector_type_nand3_axioms vector_type_nand3_def)
+
+lemma nand_seq_hoare_wityping:
+  "\<turnstile> [\<lambda>tw. nand_inv tw \<and> wityping \<Gamma> (snd tw)] (Bassign_inert C (Bnand (Bsig A) (Bsig B)) 1) [\<lambda>tw. nand_inv (next_time_world tw, snd tw) \<and> wityping \<Gamma> (snd tw)]"
+  apply (rule Conj)
+  apply (rule nand_seq_hoare_next_time_inert)
+  apply (rule strengthen_precondition2)
+  apply (rule seq_stmt_preserve_wityping_hoare)
+  apply (rule seq_wt_nand3)
+  done
+
+lemma nand_seq_hoare_next_time0_inert:
+  " \<turnstile> [\<lambda>tw. get_time tw = 0 \<and> wityping \<Gamma> (snd tw)] Bassign_inert C (Bnand (Bsig A) (Bsig B)) 1 [\<lambda>tw. nand_inv (next_time_world tw, snd tw)]"
+  apply (rule Conseq2[where Q="\<lambda>tw. nand_inv (next_time_world tw, snd tw)", rotated 1], rule AssignI2)
+  using nand_inv_next_time0_inert beval_world_raw2_type vector_type_nand3_axioms vector_type_nand3_def
+  by auto
+
+lemma nand_seq_hoare_wityping0:
+  " \<turnstile> [\<lambda>tw. get_time tw = 0 \<and> wityping \<Gamma> (snd tw)] Bassign_inert C (Bnand (Bsig A) (Bsig B)) 1 [\<lambda>tw. nand_inv (next_time_world tw, snd tw) \<and> wityping \<Gamma> (snd tw)]"
+  apply (rule Conj)
+  apply (rule nand_seq_hoare_next_time0_inert)
+  apply (rule strengthen_precondition2)
+  apply (rule seq_stmt_preserve_wityping_hoare)
+  apply (rule seq_wt_nand3)
+  done
+
+lemma nand_inv2_next_time_inert:
+  fixes tw
+  assumes "beval_world_raw2 tw (Bnand (Bsig A) (Bsig B)) v" and "type_of v = Lty len"
+  defines "tw' \<equiv> tw\<lbrakk>C, 1 :=\<^sub>2 v\<rbrakk>"
+  shows   "nand_inv2 (next_time_world tw', snd tw')"
+  unfolding nand_inv2_def
+proof (rule impI)
+  assume "disjnt {A, B} (event_of (next_time_world tw', snd tw'))"
+  let ?t' = "next_time_world tw'"
+  have "fst tw' < ?t'"
+    using next_time_world_at_least by blast
+  moreover have "fst tw = fst tw'"
+    unfolding tw'_def unfolding worldline_inert_upd2_def by auto
+  ultimately have "fst tw < ?t'"
+    by auto
+  have "wline_of tw' A ?t' = wline_of tw A ?t'"
+    unfolding tw'_def worldline_inert_upd2_def worldline_inert_upd_def by auto
+  also have "... = wline_of tw A (?t' - 1)"
+    using \<open>disjnt {A, B} (event_of (next_time_world tw', snd tw'))\<close> \<open>fst tw < ?t'\<close>
+    unfolding event_of_alt_def
+    by (simp add: tw'_def worldline_inert_upd2_def worldline_inert_upd_def)
+  also have "... = wline_of tw A (fst tw)"
+  proof -
+    have "fst tw' \<le> ?t' - 1" and "?t' - 1 < ?t'"
+      using \<open>fst tw' < ?t'\<close> by auto
+    hence "wline_of tw' A (?t' - 1) = wline_of tw' A (fst tw')"
+      using unchanged_until_next_time_world[where tw="tw'"] by blast
+    moreover have "wline_of tw' A (?t' - 1) = wline_of tw A (?t' - 1)"
+      unfolding tw'_def worldline_inert_upd2_def worldline_inert_upd_def by auto
+    moreover have "wline_of tw' A (fst tw') = wline_of tw A (fst tw')"
+      unfolding tw'_def worldline_inert_upd2_def worldline_inert_upd_def by auto
+    ultimately show ?thesis
+      using \<open>fst tw = fst tw'\<close> by auto
+  qed
+  finally have 0: "wline_of tw' A ?t' = wline_of tw A (fst tw)"
+    by auto
+  have "wline_of tw' B ?t' = wline_of tw B ?t'"
+    unfolding tw'_def worldline_inert_upd2_def worldline_inert_upd_def by auto
+  also have "... = wline_of tw B (?t' - 1)"
+    using \<open>disjnt {A, B} (event_of (next_time_world tw', snd tw'))\<close> \<open>fst tw < ?t'\<close>
+    unfolding event_of_alt_def
+    by (simp add: tw'_def worldline_inert_upd2_def worldline_inert_upd_def)
+  also have "... = wline_of tw B (fst tw)"
+  proof -
+    have "fst tw' \<le> ?t' - 1" and "?t' - 1 < ?t'"
+      using \<open>fst tw' < ?t'\<close> by auto
+    hence "wline_of tw' B (?t' - 1) = wline_of tw' B (fst tw')"
+      using unchanged_until_next_time_world[where tw="tw'"] by blast
+    moreover have "wline_of tw' B (?t' - 1) = wline_of tw B (?t' - 1)"
+      unfolding tw'_def worldline_inert_upd2_def worldline_inert_upd_def by auto
+    moreover have "wline_of tw' B (fst tw') = wline_of tw B (fst tw')"
+      unfolding tw'_def worldline_inert_upd2_def worldline_inert_upd_def by auto
+    ultimately show ?thesis
+      using \<open>fst tw = fst tw'\<close> by auto
+  qed
+  finally have 1: "wline_of tw' B ?t' = wline_of tw B (fst tw)"
+    by auto
+  { fix i
+    assume "?t' \<le> i"
+    hence "wline_of tw' C (i + 1) = v"
+    proof (cases "wline_of tw C (get_time tw) = v \<or> wline_of tw C (get_time tw + 1) \<noteq> v")
+      case True
+      thus "wline_of tw' C (i + 1) = v"
+        unfolding tw'_def worldline_inert_upd2_def worldline_inert_upd_def
+        using `fst tw < ?t'`  using \<open>next_time_world tw' \<le> i\<close> by auto
+    next
+      case False
+      let ?time = "GREATEST n. n \<le> get_time tw + 1  \<and> wline_of tw C (n - 1) \<noteq> v  \<and> wline_of tw C n = v"
+      have "?time = fst tw + 1"
+        using False by (auto intro!:Greatest_equality)
+      thus ?thesis
+        unfolding tw'_def worldline_inert_upd2_def worldline_inert_upd_def
+        using `fst tw < ?t'`  using \<open>next_time_world tw' \<le> i\<close> by auto
+    qed
+    have assms2: "beval_world_raw (snd tw) (fst tw) (Bnand (Bsig A) (Bsig B)) v"
+      using \<open>beval_world_raw2 tw (Bnand (Bsig A) (Bsig B)) v\<close> unfolding beval_world_raw2_def
+      by auto
+    have "lval_of v = map2 (\<lambda>x y. x \<longrightarrow> \<not> y) (lof_wline tw A (fst tw)) (lof_wline tw B (fst tw))"
+      apply (rule beval_world_raw_cases[OF assms2], erule beval_cases)
+      prefer 2
+      apply (metis beval_cases(1) comp_def state_of_world_def val.sel(2))
+      using assms(2) by auto
+    also have "... = map2 (\<lambda>x y. x \<longrightarrow> \<not> y) (lof_wline tw' A ?t') (lof_wline tw' B ?t')"
+      using 0 1 by auto
+    finally have "lof_wline tw' C (i + 1) = map2 (\<lambda>x y. x \<longrightarrow> \<not> y) (lof_wline tw' A ?t') (lof_wline tw' B ?t')"
+      using \<open>wline_of tw' C (i + 1) = v\<close> by blast }
+  thus "\<forall>i\<ge>get_time (next_time_world tw', snd tw').
+       lof_wline (next_time_world tw', snd tw') C (i + 1) =
+       map2 (\<lambda>x y. x \<longrightarrow> \<not> y) (lof_wline (next_time_world tw', snd tw') A (get_time (next_time_world tw', snd tw')))
+        (lof_wline (next_time_world tw', snd tw') B (get_time (next_time_world tw', snd tw')))"
+    by auto
+qed
+
+lemma nand_seq_hoare_next_time4_inert:
+  " \<turnstile> [\<lambda>tw. wityping \<Gamma> (snd tw)] Bassign_inert C (Bnand (Bsig A) (Bsig B)) 1 [\<lambda>tw. nand_inv2 (next_time_world tw, snd tw)]"
+  apply (rule Conseq2[where Q="\<lambda>tw. nand_inv2 (next_time_world tw, snd tw)", rotated 1], rule AssignI2, blast)
+  using nand_inv2_next_time_inert beval_world_raw2_type vector_type_nand3_axioms vector_type_nand3_def
+  by auto
+
+lemma nand_seq_hoare2_wityping:
+  " \<turnstile> [\<lambda>tw. wityping \<Gamma> (snd tw)] Bassign_inert C (Bnand (Bsig A) (Bsig B)) 1 [\<lambda>tw. nand_inv2 (next_time_world tw, snd tw) \<and> wityping \<Gamma> (snd tw)]"
+  apply (rule Conj)
+  apply (rule nand_seq_hoare_next_time4_inert)
+  apply (rule seq_stmt_preserve_wityping_hoare)
+  apply (rule seq_wt_nand3)
+  done
+
+lemma nand_conc_hoare3_inert_without:
+  "\<turnstile> \<lbrace>\<lambda>tw. (nand_inv tw \<and> wityping \<Gamma> (snd tw)) \<and> nand_inv2 tw\<rbrace> nand \<lbrace>\<lambda>tw. nand_inv (next_time_world tw, snd tw)  \<and> nand_inv2  (next_time_world tw, snd tw)\<rbrace>"
+  unfolding nand_def
+  apply (rule Single)
+   apply (rule Conj)
+    apply (rule strengthen_precondition)
+    apply (rule strengthen_precondition)
+    apply(rule weaken_postcondition[OF nand_seq_hoare_wityping])
+   apply (rule strengthen_precondition)
+   apply (rule strengthen_precondition)
+   apply (rule strengthen_precondition2)
+   apply(rule weaken_postcondition[OF nand_seq_hoare2_wityping])
+  using nand_conc_hoare' nand_conc_hoare2 by blast
+
+lemma nand_preserve_wityping:
+  " \<turnstile> \<lbrace>\<lambda>tw. wityping \<Gamma> (snd tw)\<rbrace> nand \<lbrace>\<lambda>tw. wityping \<Gamma> (snd tw)\<rbrace>"
+  unfolding nand_def using single_conc_stmt_preserve_wityping_hoare
+  using conc_wt.intros(1) seq_wt_nand3
+  by (simp add: single_conc_stmt_preserve_wityping_hoare)
+
+lemma nand_conc_hoare3_inert:
+  "\<turnstile> \<lbrace>\<lambda>tw. (nand_inv tw \<and> wityping \<Gamma> (snd tw)) \<and> nand_inv2 tw\<rbrace> nand \<lbrace>\<lambda>tw. (nand_inv (next_time_world tw, snd tw) \<and> wityping \<Gamma> (snd tw)) \<and> nand_inv2  (next_time_world tw, snd tw)\<rbrace>"
+  apply (rule Conj2)
+   apply (rule Conj2)
+    apply (rule weaken_post_conc_hoare[rotated])
+  apply (rule nand_conc_hoare3_inert_without, blast)
+   apply (rule strengthen_pre_conc_hoare[rotated])
+    apply (rule nand_preserve_wityping)
+   apply blast
+  apply (rule weaken_post_conc_hoare[rotated])
+   apply (rule nand_conc_hoare3_inert_without, blast)
+  done
+
+lemma nand_conc_sim'_inert:
+  "\<turnstile>\<^sub>s \<lbrace>\<lambda>tw. (nand_inv tw \<and> wityping \<Gamma> (snd tw)) \<and> nand_inv2 tw\<rbrace> nand \<lbrace>\<lambda>tw. (nand_inv tw \<and> wityping \<Gamma> (snd tw)) \<and> nand_inv2 tw\<rbrace>"
+  apply (rule While)
+  unfolding snd_conv apply (rule nand_conc_hoare3_inert)
+  done
+
+lemma nand_conc_sim2'_inert:
+  "\<turnstile>\<^sub>s \<lbrace>\<lambda>tw. (nand_inv tw \<and> wityping \<Gamma> (snd tw)) \<and> nand_inv2 tw\<rbrace> nand \<lbrace>\<lambda>tw. nand_inv tw \<and> wityping \<Gamma> (snd tw)\<rbrace>"
+  apply (rule Conseq_sim[rotated])
+    apply (rule nand_conc_sim'_inert)
+  by blast+
+
+lemma init_sat_nand_inv_inert:
+  "init_sim_hoare (\<lambda>tw. fst tw = 0 \<and> wityping \<Gamma> (snd tw)) nand (\<lambda>tw. nand_inv tw \<and> wityping \<Gamma> (snd tw))"
+  unfolding nand_def
+  apply (rule AssignI)
+  apply (rule SingleI)
+  unfolding snd_conv apply (rule nand_seq_hoare_wityping0)
+  done
+
+lemma init_sat_nand_inv2_inert:
+  "init_sim_hoare (\<lambda>tw. wityping \<Gamma> (snd tw)) nand (\<lambda>tw. nand_inv2 tw \<and> wityping \<Gamma> (snd tw))"
+  unfolding nand_def
+  apply (rule AssignI)
+  apply (rule SingleI)
+  unfolding snd_conv  apply (rule nand_seq_hoare2_wityping)
+  done
+
+lemma init_sat_nand_inv_comb_inert:
+  "init_sim_hoare (\<lambda>tw. fst tw = 0 \<and> wityping \<Gamma> (snd tw)) nand (\<lambda>tw. (nand_inv tw \<and> wityping \<Gamma> (snd tw)) \<and> nand_inv2 tw)"
+  apply (rule ConjI_sim)
+  apply (rule init_sat_nand_inv_inert)
+  apply (rule ConseqI_sim[where P="\<lambda>tw. wityping \<Gamma> (snd tw)" and Q="\<lambda>tw. nand_inv2 tw \<and> wityping \<Gamma> (snd tw)"])
+  apply (simp, rule init_sat_nand_inv2_inert, simp)
+  done
+
+lemma nand_correctness_inert:
+  assumes "sim_fin w (i + 1) nand tw'" and "wityping \<Gamma> w"
+  shows   "lof_wline tw' C (i + 1) = map2 (\<lambda>x y. x \<longrightarrow> \<not> y) (lof_wline tw' A i) (lof_wline tw' B i)"
+proof -
+  obtain tw where "init_sim (0, w) nand tw" and  "tw, i + 1, nand \<Rightarrow>\<^sub>S tw'"
+    using premises_sim_fin_obt[OF assms(1)] by auto
+  hence "i + 1 < fst tw'"
+    using world_maxtime_lt_fst_tres  by blast
+  have "conc_stmt_wf nand"
+    unfolding conc_stmt_wf_def nand_def by auto
+  moreover have "nonneg_delay_conc nand"
+    unfolding nand_def by auto
+  ultimately have "init_sim_valid (\<lambda>tw. fst tw = 0 \<and> wityping \<Gamma> (snd tw)) nand (\<lambda>tw. (nand_inv tw \<and> wityping \<Gamma> (snd tw)) \<and> nand_inv2 tw)"
+    using init_sim_hoare_soundness[OF init_sat_nand_inv_comb_inert] by auto
+  hence "nand_inv tw \<and> nand_inv2 tw \<and> wityping \<Gamma> (snd tw)"
+    using \<open>init_sim (0, w) nand tw\<close> fst_conv assms(2) unfolding init_sim_valid_def
+    by (metis snd_conv)
+  hence "nand_inv tw" and "nand_inv2 tw" and "wityping \<Gamma> (snd tw)"
+    by auto
+  moreover have "\<Turnstile>\<^sub>s \<lbrace>\<lambda>tw. (nand_inv tw \<and> wityping \<Gamma> (snd tw)) \<and> nand_inv2 tw\<rbrace> nand \<lbrace>\<lambda>tw. nand_inv tw \<and> wityping \<Gamma> (snd tw)\<rbrace>"
+    using conc_sim_soundness[OF nand_conc_sim2'_inert] \<open>conc_stmt_wf nand\<close> \<open>nonneg_delay_conc nand\<close>
+    by auto
+  ultimately have "nand_inv tw' \<and> wityping \<Gamma> (snd tw')"
+    using \<open>tw, i + 1, nand \<Rightarrow>\<^sub>S tw'\<close> unfolding sim_hoare_valid_def by blast
+  hence "\<forall>i < fst tw'. lof_wline tw' C (i + 1) = map2 (\<lambda>x y. x \<longrightarrow> \<not> y) (lof_wline tw' A i) (lof_wline tw' B i)"
+    unfolding nand_inv_def by auto
+  with \<open>i + 1 < fst tw'\<close> show ?thesis
+    by auto
+qed
+
+end
+
+lemma tyenv_possibilities_bexp_wt:
+  assumes " bexp_wt \<Gamma>' (Bnand (Bsig A) (Bsig B)) (\<Gamma>' C) "
+  shows "\<exists>len. \<Gamma>' A = Bty \<and> \<Gamma>' B = Bty \<and> \<Gamma>' C = Bty \<or> \<Gamma>' A = Lty len \<and> \<Gamma>' B = Lty len \<and> \<Gamma>' C = Lty len"
+proof (rule bexp_wt_cases(4)[OF assms])
+  assume "bexp_wt \<Gamma>' (Bsig A) (\<Gamma>' C)"
+  hence "\<Gamma>' C = \<Gamma>' A"
+    using bexp_wt.cases by auto
+  assume "bexp_wt \<Gamma>' (Bsig B) (\<Gamma>' C)"
+  hence "\<Gamma>' C = \<Gamma>' B"
+    using bexp_wt.cases by auto
+  obtain len where "\<Gamma>' C = Bty \<or> \<Gamma>' C = Lty len"
+    using ty.exhaust by auto
+  moreover
+  { assume "\<Gamma>' C = Bty"
+    hence "\<Gamma>' A = Bty" and "\<Gamma>' B = Bty"
+      using \<open>\<Gamma>' C = \<Gamma>' A\<close> \<open>\<Gamma>' C = \<Gamma>' B\<close> by auto
+    hence "\<exists>len. \<Gamma>' A = Bty \<and> \<Gamma>' B = Bty \<and> \<Gamma>' C = Bty \<or> \<Gamma>' A = Lty len \<and> \<Gamma>' B = Lty len \<and> \<Gamma>' C = Lty len"
+      apply (intro exI[where x="len"])
+      using \<open>\<Gamma>' C = Bty\<close> by auto }
+  moreover
+  { assume "\<Gamma>' C = Lty len"
+    hence "\<Gamma>' A = Lty len" and "\<Gamma>' B = Lty len"
+      using \<open>\<Gamma>' C = \<Gamma>' A\<close> \<open>\<Gamma>' C = \<Gamma>' B\<close> by auto
+    hence "\<exists>len. \<Gamma>' A = Bty \<and> \<Gamma>' B = Bty \<and> \<Gamma>' C = Bty \<or> \<Gamma>' A = Lty len \<and> \<Gamma>' B = Lty len \<and> \<Gamma>' C = Lty len"
+      apply (intro exI[where x="len"])
+      using \<open>\<Gamma>' C = Lty len\<close> by auto }
+  ultimately show ?thesis
+    by auto
+qed
+
+lemma tyenv_possibilities_seq_wt:
+  assumes "seq_wt \<Gamma>' (Bassign_trans C (Bnand (Bsig A) (Bsig B)) 1)"
+  shows "\<exists>len. \<Gamma>' A = Bty \<and> \<Gamma>' B = Bty \<and> \<Gamma>' C = Bty \<or> \<Gamma>' A = Lty len \<and> \<Gamma>' B = Lty len \<and> \<Gamma>' C = Lty len"
+  apply (rule seq_wt_cases(4)[OF assms])
+  apply (rule tyenv_possibilities_bexp_wt)
+  by simp
+
+lemma tyenv_possibilities_conc_wt:
+  assumes "conc_wt \<Gamma>' nand3"
+  shows "\<exists>len. \<Gamma>' A = Bty \<and> \<Gamma>' B = Bty \<and> \<Gamma>' C = Bty \<or> \<Gamma>' A = Lty len \<and> \<Gamma>' B = Lty len \<and> \<Gamma>' C = Lty len"
+  using assms unfolding nand3_def
+  by (metis conc_stmt.sel(4) conc_stmt.simps(4) conc_wt.cases tyenv_possibilities_seq_wt)
+
+theorem nand3_correctness:
+  assumes "conc_wt \<Gamma>' nand3"
+  assumes "sim_fin w (i + 1) nand3 tw'" and "wityping \<Gamma>' w"
+  shows   " (\<Gamma>' A \<noteq> Bty \<longrightarrow> lof_wline tw' C (i + 1) = map2 (\<lambda>x y. x \<longrightarrow> \<not> y) (lof_wline tw' A i)  (lof_wline tw' B i))
+          \<or> (\<Gamma>' A = Bty \<longrightarrow> bval_of_wline tw' C (i + 1) \<longleftrightarrow> \<not> (bval_of_wline tw' A i \<and> bval_of_wline tw' B i))"
+proof -
+  obtain len where "\<Gamma>' A = Bty \<and> \<Gamma>' B = Bty \<and> \<Gamma>' C = Bty \<or> \<Gamma>' A = Lty len \<and> \<Gamma>' B = Lty len \<and> \<Gamma>' C = Lty len"
+    using tyenv_possibilities_conc_wt[OF assms(1)] by auto
+  moreover
+  { assume "\<Gamma>' A = Bty \<and> \<Gamma>' B = Bty \<and> \<Gamma>' C = Bty"
+    then interpret l1: scalar_type_nand3 \<Gamma>' unfolding scalar_type_nand3_def .
+    have "bval_of_wline tw' C (i + 1) \<longleftrightarrow> \<not> (bval_of_wline tw' A i \<and> bval_of_wline tw' B i)"
+      using l1.nand_correctness[OF assms(2-3)] by auto
+    hence ?thesis
+      using \<open>\<Gamma>' A = Bty \<and> \<Gamma>' B = Bty \<and> \<Gamma>' C = Bty\<close> by auto }
+  moreover
+  { assume "\<Gamma>' A = Lty len \<and> \<Gamma>' B = Lty len \<and> \<Gamma>' C = Lty len"
+    then interpret l2: vector_type_nand3 len \<Gamma>'
+      by unfold_locales auto
+    have "lof_wline tw' C (i + 1) = map2 (\<lambda>x y. x \<longrightarrow> \<not> y) (lof_wline tw' A i)  (lof_wline tw' B i)"
+      using l2.nand_correctness[OF assms(2-3)] by auto
+    hence ?thesis
+      using \<open>\<Gamma>' A = Lty len \<and> \<Gamma>' B = Lty len \<and> \<Gamma>' C = Lty len\<close> by auto }
+  ultimately show ?thesis
+    by auto
+qed
+
+lemma tyenv_possibilities_seq_wt_inert:
+  assumes "seq_wt \<Gamma>' (Bassign_inert C (Bnand (Bsig A) (Bsig B)) 1)"
+  shows "\<exists>len. \<Gamma>' A = Bty \<and> \<Gamma>' B = Bty \<and> \<Gamma>' C = Bty \<or> \<Gamma>' A = Lty len \<and> \<Gamma>' B = Lty len \<and> \<Gamma>' C = Lty len"
+  apply (rule seq_wt_cases(5)[OF assms])
+  apply (rule tyenv_possibilities_bexp_wt)
+  by simp
+
+lemma tyenv_possibilities_conc_wt_inert:
+  assumes "conc_wt \<Gamma>' nand"
+  shows "\<exists>len. \<Gamma>' A = Bty \<and> \<Gamma>' B = Bty \<and> \<Gamma>' C = Bty \<or> \<Gamma>' A = Lty len \<and> \<Gamma>' B = Lty len \<and> \<Gamma>' C = Lty len"
+  using assms unfolding nand_def
+  by (metis conc_stmt.distinct(1) conc_stmt.sel(4) conc_wt.cases tyenv_possibilities_seq_wt_inert)
+
+theorem nand_correctness:
+  assumes "conc_wt \<Gamma>' nand"
+  assumes "sim_fin w (i + 1) nand3 tw'" and "wityping \<Gamma>' w"
+  shows   " (\<Gamma>' A \<noteq> Bty \<longrightarrow> lof_wline tw' C (i + 1) = map2 (\<lambda>x y. x \<longrightarrow> \<not> y) (lof_wline tw' A i)  (lof_wline tw' B i))
+          \<or> (\<Gamma>' A = Bty \<longrightarrow> bval_of_wline tw' C (i + 1) \<longleftrightarrow> \<not> (bval_of_wline tw' A i \<and> bval_of_wline tw' B i))"
+proof -
+  obtain len where "\<Gamma>' A = Bty \<and> \<Gamma>' B = Bty \<and> \<Gamma>' C = Bty \<or> \<Gamma>' A = Lty len \<and> \<Gamma>' B = Lty len \<and> \<Gamma>' C = Lty len"
+    using tyenv_possibilities_conc_wt_inert[OF assms(1)] by auto
+  moreover
+  { assume "\<Gamma>' A = Bty \<and> \<Gamma>' B = Bty \<and> \<Gamma>' C = Bty"
+    then interpret l1: scalar_type_nand3 \<Gamma>' unfolding scalar_type_nand3_def .
+    have "bval_of_wline tw' C (i + 1) \<longleftrightarrow> \<not> (bval_of_wline tw' A i \<and> bval_of_wline tw' B i)"
+      using l1.nand_correctness[OF assms(2-3)] by auto
+    hence ?thesis
+      using \<open>\<Gamma>' A = Bty \<and> \<Gamma>' B = Bty \<and> \<Gamma>' C = Bty\<close> by auto }
+  moreover
+  { assume "\<Gamma>' A = Lty len \<and> \<Gamma>' B = Lty len \<and> \<Gamma>' C = Lty len"
+    then interpret l2: vector_type_nand3 len \<Gamma>'
+      by unfold_locales auto
+    have "lof_wline tw' C (i + 1) = map2 (\<lambda>x y. x \<longrightarrow> \<not> y) (lof_wline tw' A i)  (lof_wline tw' B i)"
+      using l2.nand_correctness[OF assms(2-3)] by auto
+    hence ?thesis
+      using \<open>\<Gamma>' A = Lty len \<and> \<Gamma>' B = Lty len \<and> \<Gamma>' C = Lty len\<close> by auto }
+  ultimately show ?thesis
     by auto
 qed
 
